implementing shared references

Rustv/Rustv.thy
@@ -7,7 +7,7 @@ datatype rust_error = invalid_ref
 datatype pointer = ptr_val nat
 datatype tag = tag_val nat
 datatype val = int_val int
-record tagged_ref = 
+record tagged_ref =
   pointer :: pointer
   tag :: tag
 
@@ -17,111 +17,186 @@ fun the_ptr :: "pointer \<Rightarrow> nat" where
 fun the_tag :: "tag \<Rightarrow> nat" where
   "the_tag (tag_val t) = t"
 
+datatype ref_kind = Unique | SharedReadWrite | SharedReadOnly
+type_synonym 'a stack = "'a list"
+
 record globals_ram =
   memory :: "val list"
-  tags :: "tag list list" (* `tag set list list` in the presence of shared pointer *)
+  tags :: "(ref_kind * tag set) stack list"
   issued_tags :: "tag list"
 
-fun wf_tags :: "tag list list \<Rightarrow> bool" where
+inductive wf_reborrow :: "(ref_kind * tag set) stack \<Rightarrow> bool" where
+  (* An allocation root is a Unique reference (Box) *)
+  BorrowRoot: "wf_reborrow [(Unique, {t})]" |
+
+  (* Reborrowing from a Unique reference *)
+  ReborrowUniqueUnique:
+    "wf_reborrow ((Unique, {t}) # tail) \<Longrightarrow> wf_reborrow ((Unique, {t'}) # (Unique, {t}) # tail)" |
+  ReborrowUniqueSRW:
+    "wf_reborrow ((Unique, {t}) # tail) \<Longrightarrow> wf_reborrow ((SharedReadWrite, ts) # (Unique, {t}) # tail)" |
+  ReborrowUniqueSRO:
+    "wf_reborrow ((Unique, {t}) # tail) \<Longrightarrow> wf_reborrow ((SharedReadOnly, ts) # (Unique, {t}) # tail)" |
+
+  (* Reborrowing from a SharedReadWrite *)
+  ReborrowSRWUnique:
+    "wf_reborrow ((SharedReadWrite, ts) # tail)
+ \<Longrightarrow> wf_reborrow ((Unique, {t'}) # (SharedReadWrite, ts) # tail)" |
+  ReborrowSRWSRW:
+    "wf_reborrow ((SharedReadWrite, ts) # tail)
+ \<Longrightarrow> wf_reborrow ((SharedReadWrite, insert t ts) # tail)" |
+  ReborrowSRWSRO:
+    "wf_reborrow ((SharedReadWrite, ts) # tail)
+ \<Longrightarrow> wf_reborrow ((SharedReadOnly, ts') # (SharedReadWrite, ts) # tail)" |
+
+  (* Reborrowing from a SharedReadOnly gives only a shared reference *)
+  ReborrowSROSRO:
+    "wf_reborrow ((SharedReadOnly, ts) # tail)
+ \<Longrightarrow> wf_reborrow ((SharedReadOnly, insert t ts) # tail)"
+
+inductive_cases wf_reborrow_elims: "wf_reborrow stack"
+
+lemma wf_reborrow_nonempty:
+  assumes "wf_reborrow stack"
+  shows "stack \<noteq> []"
+using assms proof (rule wf_reborrow_elims)
+qed auto
+
+lemma wf_reborrow_root: "wf_reborrow stack \<Longrightarrow> \<exists>t. last stack = (Unique, {t})"
+proof (induction rule: wf_reborrow.induct)
+qed auto
+
+lemma unique_ref_head:
+  assumes "wf_reborrow ((Unique, ts) # end)"
+  shows "\<exists>t. ts = {t}"
+using assms proof (rule wf_reborrow_elims)
+qed auto
+
+lemma unique_ref:
+  assumes
+    "wf_reborrow stack"
+    "(Unique, ts) \<in> set stack"
+  shows "\<exists>t. ts = {t}"
+using assms(1) assms(2) proof (induction rule: wf_reborrow.induct)
+qed auto
+
+lemma wf_reborrow_pop:
+  assumes
+    "wf_reborrow stack"
+    "stack = st1 # st2 # rest"
+  shows "wf_reborrow (st2 # rest)"
+using assms proof (induction arbitrary: st1 rule: wf_reborrow.induct)
+qed auto
+
+lemma wf_reborrow_pop':
+  fixes top rest
+  assumes
+    "wf_reborrow (top # rest)"
+    "rest \<noteq> []"
+  shows "wf_reborrow rest"
+using assms proof (induction "(top # rest)" arbitrary: top rule: wf_reborrow.induct)
+qed auto
+
+fun stack_finite :: "(ref_kind * tag set) stack \<Rightarrow> bool" where
+  "stack_finite [] = True" |
+  "stack_finite (s # stack) = (finite (snd s) \<and> stack_finite stack)"
+
+lemma stack_finite_spec: "stack_finite stack \<longleftrightarrow> (\<forall>s \<in> set stack. finite (snd s))"
+proof (induction stack)
+qed auto
+
+fun wf_tags :: "(ref_kind * tag set) stack list \<Rightarrow> bool" where
   "wf_tags [] = True" |
-  "wf_tags ([] # _) = False" |
-  "wf_tags (_ # t) = wf_tags t"
-lemma wf_tags_spec: "wf_tags ts \<longleftrightarrow> (\<forall>t \<in> set ts. t \<noteq> [])"
+  "wf_tags (stack # ts) = (wf_reborrow stack \<and> stack_finite stack \<and> wf_tags ts)"
+
+lemma wf_tags_spec:
+  "wf_tags ts \<longleftrightarrow> (\<forall>stack \<in> set ts. wf_reborrow stack \<and> stack_finite stack)"
 proof (induction ts)
-  case Nil
-  then show ?case by simp
-next
-  case (Cons a ts)
+qed auto
 
-  have 1: "wf_tags (a # ts) \<Longrightarrow> (\<forall>t \<in> set (a # ts). t \<noteq> [])"
-  proof (cases "a # ts" rule: wf_tags.elims(2))
-    show "wf_tags (a # ts) \<Longrightarrow> wf_tags (a # ts)" by simp
-  next
-    fix v tail
-
-    assume "wf_tags ts"
-    then have "\<forall>t \<in> set ts. t \<noteq> []" using Cons.IH by auto
-    moreover assume "a = v # tail"
-    thus ?thesis using calculation by auto
-  qed
-
-  have 2: "(\<forall>t \<in> set (a # ts). t \<noteq> []) \<Longrightarrow> wf_tags (a # ts)"
-    using Cons.IH wf_tags.elims(3) by fastforce
-
-  show ?case using 1 2 by (rule iffI)
-qed
-
-lemma [simp, intro]: "\<lbrakk>wf_tags ts; x \<noteq> []\<rbrakk> \<Longrightarrow> wf_tags (ts @ [x])"
-proof (induction ts)
-  case Nil
-  then show ?case by (simp add: wf_tags_spec)
-next
-  case (Cons a ts)
-  then show ?case by (simp add: wf_tags_spec)
-qed
+lemma list_update_forall:
+  "\<lbrakk>\<forall>x \<in> set xs. P x; P x'\<rbrakk> \<Longrightarrow> \<forall>x \<in> set (xs[p := x']). P x"
+  using set_update_subset_insert by fastforce
 
 lemma wf_tags_update:
   assumes
-    "wf_tags tag_stack"
-    "ts \<noteq> []"
-  shows
-    "wf_tags (tag_stack[p := ts])"
-  using assms(1) assms(2) set_update_subset_insert wf_tags_spec by fastforce
+    "wf_tags ts"
+    "wf_reborrow stack"
+    "stack_finite stack"
+  shows "wf_tags (ts[p := stack])"
+  using assms set_update_subset_insert wf_tags_spec by fastforce
 
-fun collect_tags :: "tag list list \<Rightarrow> tag set" where
-  "collect_tags ts = foldr (\<lambda>ts accum. set ts \<union> accum) ts {}"
-lemma collect_tags_spec: "t \<in> collect_tags ts \<longleftrightarrow> (\<exists>i < length ts. t \<in> set (ts ! i))"
+fun collect_tags_stack :: "(ref_kind * tag set) stack \<Rightarrow> tag set" where
+  "collect_tags_stack stack = \<Union>(set (map snd stack))"
+
+fun collect_tags :: "(ref_kind * tag set) stack list \<Rightarrow> tag set" where
+  "collect_tags [] = {}" |
+  "collect_tags (stack # ts) = collect_tags_stack stack \<union> collect_tags ts"
+lemma collect_tags_spec:
+  "t \<in> collect_tags ts \<longleftrightarrow> (\<exists>stack \<in> set ts. \<exists>entry \<in> set (map snd stack). t \<in> entry)"
 proof (induction ts)
   case Nil
   then show ?case by simp
 next
-  case (Cons h ts)
-  have 1: "collect_tags (h # ts) = set h \<union> collect_tags ts" by simp
-
+  case (Cons stack ts)
   show ?case
   proof
-    assume "t \<in> collect_tags (h # ts)"
-    then have 2: "t \<in> set h \<or> t \<in> collect_tags ts" using 1 by simp
-    thus "\<exists>i < length (h # ts). t \<in> set ((h # ts) ! i)"
-    proof (cases rule: disjE[OF 2])
-      case 1
-      then show ?thesis by auto
+    assume "t \<in> collect_tags (stack # ts)"
+    then have "t \<in> \<Union>(set (map snd stack)) \<or> t \<in> collect_tags ts" by simp
+    then show "\<exists>s \<in> set (stack # ts). \<exists>entry \<in> set (map snd s). t \<in> entry"
+    proof (rule disjE)
+      assume "t \<in> \<Union>(set (map snd stack))"
+      then show ?thesis by simp
     next
-      case 2
-      then show ?thesis using Cons.IH by auto
+      assume "t \<in> collect_tags ts"
+      then show ?thesis by (simp add: Cons.IH)
     qed
   next
-    assume "\<exists>i < length (h # ts). t \<in> set ((h # ts) ! i)"
-    then obtain i where
-      3: "i < length (h # ts)" and
-      4: "t \<in> set ((h # ts) ! i)"
+    assume "\<exists>stack \<in> set (stack # ts). \<exists>entry \<in> set (map snd stack). t \<in> entry"
+    then obtain s entry where
+      1: "s \<in> set (stack # ts)" and
+      2: "entry \<in> set (map snd s)" and
+      3: "t \<in> entry"
       by auto
-    thus "t \<in> collect_tags (h # ts)"
-    proof (cases "i = 0")
-      case True
-      then show ?thesis using 4 by auto
+
+    have "s = stack \<or> s \<in> set ts" using 1 by auto
+    then show "t \<in> collect_tags (stack # ts)"
+    proof (rule disjE)
+      assume "s = stack"
+      then have "\<exists>entry \<in> set (map snd stack). t \<in> entry" using 2 3 by auto
+      then show ?thesis by simp
     next
-      case False
-      then have "t \<in> set (ts ! (i - 1))" using 4 by auto
-      then show ?thesis using 3 Cons.IH \<open>i \<noteq> 0\<close> by auto
+      assume "s \<in> set ts"
+      then have "\<exists>s \<in> set ts. \<exists>entry \<in> set (map snd s). t \<in> entry"
+        using 2 3 by auto
+      then show ?thesis by (simp add: Cons.IH)
     qed
   qed
 qed
 
-(* sometimes collect_tags.simps confuses the automatic reasoner *)
-declare collect_tags.simps[simp del]
+lemma collect_tags_spec':
+  "t \<in> collect_tags ts \<longleftrightarrow> (\<exists>stack \<in> set ts. t \<in> collect_tags_stack stack)"
+  using collect_tags_spec by fastforce
 
 lemma collect_tags_update[simp, intro]:
-  "t \<in> collect_tags (ts[p := x]) \<Longrightarrow> t \<in> collect_tags ts \<or> t \<in> set x"
-  by (metis collect_tags_spec length_list_update nth_list_update nth_list_update_neq)
+  "t \<in> collect_tags (ts[p := stack]) \<Longrightarrow> t \<in> collect_tags ts \<or> t \<in> collect_tags_stack stack"
+  using collect_tags_spec set_update_subset_insert subset_code(1) by fastforce
 
-lemma [simp, intro]: "collect_tags (ts @ [t]) = set t \<union> (collect_tags ts)"
+lemma collect_tags_last[simp, intro]:
+  "collect_tags (ts @ [stack]) = collect_tags_stack stack \<union> (collect_tags ts)"
 proof (induction ts)
-qed (auto simp add: collect_tags.simps)
+qed auto
 
-lemma [simp, intro]: "finite (collect_tags ts)"
+lemma collect_tags_stack_finite:
+  assumes "stack_finite stack"
+  shows "finite (collect_tags_stack stack)"
+  using assms stack_finite_spec by auto
+
+lemma collect_tags_finite[simp, intro]: "wf_tags ts \<Longrightarrow> finite (collect_tags ts)"
 proof (induction ts)
-qed (simp add: collect_tags.simps)+
+  case (Cons stack ts)
+  then have "stack_finite stack \<and> finite (collect_tags ts)" by auto
+  then show ?case using collect_tags_stack_finite by auto
+qed auto
 
 fun wf_heap :: "'a globals_ram_scheme \<Rightarrow> bool" where
   "wf_heap s \<longleftrightarrow>
@@ -131,26 +206,61 @@ fun wf_heap :: "'a globals_ram_scheme \<Rightarrow> bool" where
 
 (* when we use a unique reference, invalidate all children *)
 fun invalidate_children :: "tagged_ref \<Rightarrow> 'a globals_ram_scheme \<Rightarrow> 'a globals_ram_scheme" where
-  "invalidate_children r s = 
+  "invalidate_children r s =
     (let p = the_ptr (pointer r);
-         ts = tags s ! p;
-         ts' = dropWhile ((\<noteq>) (tag r)) ts in
-    s\<lparr> tags := (tags s)[p := ts'] \<rparr>)"
+         stack = tags s ! p;
+         stack' = dropWhile (\<lambda>entry. (tag r) \<notin> snd entry) stack in
+    s\<lparr> tags := (tags s)[p := stack'] \<rparr>)"
 
 fun_cases invalidate_childrenE: "invalidate_children r s = s'"
 
-lemma dropWhile_hd_eq[simp, intro]: "x \<in> set xs \<Longrightarrow> hd (dropWhile ((\<noteq>) x) xs) = x"
-proof (induction xs)
-qed auto
+lemma hd_dropWhile_stack:
+  assumes
+    "dropWhile (\<lambda>entry. (tag r) \<notin> snd entry) stack = stack'"
+    "\<exists>entry \<in> set stack. (tag r) \<in> snd entry"
+  shows "tag r \<in> snd (hd stack')"
+  by (metis assms(1) assms(2) dropWhile_eq_Nil_conv hd_dropWhile)
 
-lemma dropWhile_in[simp, intro]: "x \<in> set xs \<Longrightarrow> x \<in> set (dropWhile ((\<noteq>) x) xs)"
-proof (induction xs)
-qed auto
+lemma dropWhile_stack_reborrow:
+  "wf_reborrow stack \<and> dropWhile P stack \<noteq> [] \<Longrightarrow> wf_reborrow (dropWhile P stack)"
+proof (induction stack)
+  case Nil
+  then show ?case using wf_reborrow_nonempty by simp
+next
+  case (Cons top rest)
 
-lemma "\<lbrakk>invalidate_children r s = s'; the_ptr (pointer r) < length (tags s); tag r \<in> set ((tags s') ! the_ptr (pointer r))\<rbrakk>
-  \<Longrightarrow> hd ((tags s') ! the_ptr (pointer r)) = tag r"
-  apply (erule invalidate_childrenE)
-  by (simp add: Let_def set_dropWhileD)
+  show ?case
+  proof (cases "P top")
+    case True
+    moreover have "dropWhile P rest \<noteq> []" using Cons.prems calculation by auto
+    moreover have "rest \<noteq> []" using calculation by auto
+    moreover have "wf_reborrow rest" using calculation Cons.prems wf_reborrow_pop' by auto
+    ultimately show ?thesis using Cons.IH by auto
+  next
+    case False
+    then have "dropWhile P (top # rest) = top # rest" by simp
+    then show ?thesis using Cons.prems by simp
+  qed
+qed
+(*
+lemma invalidate_wf_tags:
+  assumes
+    "invalidate_children r s = s'"
+    "\<exists>entry \<in> set ((tags s) ! the_ptr (pointer r)). (tag r) \<in> snd entry"
+    "wf_tags (tags s)"
+  shows "wf_tags (tags s')"
+  sorry
+
+lemma
+  assumes
+    "invalidate_children r s = s'"
+    "wf_tags (tags s)"
+    "the_ptr (pointer r) < length (tags s)"
+    "tag r \<in> collect_tag_stack ((tags s') ! the_ptr (pointer r))"
+  shows "tag r \<in> snd (hd ((tags s') ! the_ptr (pointer r)))"
+  using assms(1) apply (rule invalidate_childrenE)
+  apply (simp add: Let_def)
+  by (simp add: Let_def set_dropWhileD) *)
 
 lemma invalidate_children_memory[intro]:
   "invalidate_children r s = s' \<Longrightarrow> memory s' = memory s"
@@ -216,34 +326,38 @@ lemma new_tag_notin_at:
     "wf_heap s"
     "new_tag s = t"
     "r < length (tags s)"
-  shows "t \<notin> set (tags s ! r)"
+  shows "t \<notin> collect_tags_stack (tags s ! r)"
 proof -
   have "t \<notin> set (issued_tags s)" using assms by auto
   then have "t \<notin> collect_tags (tags s)" using assms by auto
-  then have "\<not>(\<exists>i < length (tags s). t \<in> set ((tags s) ! i))"
-    using collect_tags_spec by auto
-  thus ?thesis using assms by auto
+  thus ?thesis using assms using collect_tags_spec' nth_mem by blast
 qed
 
+fun writable_stack :: "tag \<Rightarrow> (ref_kind * tag set) stack \<Rightarrow> bool" where
+  "writable_stack t [] \<longleftrightarrow> False" |
+  "writable_stack t ((Unique, ts) # stack) \<longleftrightarrow> t \<in> ts \<or> writable_stack t stack" |
+  "writable_stack t ((SharedReadWrite, ts) # stack) \<longleftrightarrow> t \<in> ts \<or> writable_stack t stack" |
+  "writable_stack t ((SharedReadOnly, ts) # stack) \<longleftrightarrow> writable_stack t stack"
+
 fun writable :: "tagged_ref \<Rightarrow> 'a globals_ram_scheme \<Rightarrow> bool" where
-  "writable r s = 
+  "writable r s =
     (let p = the_ptr (pointer r) in
     let t = tag r in
-    p < length (memory s) \<and> t \<in> set (tags s ! p))"
+    p < length (memory s) \<and> writable_stack t (tags s ! p))"
 
 lemma writable_update[simp]: "writable r (memwrite r' v s) = writable r s"
-  by auto
+  by simp
 
 lemma writable_invalidated[intro]: "writable r s \<Longrightarrow> writable r (invalidate_children r s)"
   apply (simp add: Let_def)
-  apply auto
-  by (metis dropWhile_in list_update_beyond not_le nth_list_update_eq)
+  apply (auto simp add: nth_list_update_eq)
+  by (metis dropWhile_in list_update_beyond not_le nth_list_updateeq)
 
 fun new_pointer :: "'a globals_ram_scheme \<Rightarrow> pointer" where
   "new_pointer s = ptr_val (length (memory s))"
 
 fun heap_new :: "val \<Rightarrow> 'a globals_ram_scheme \<Rightarrow> tagged_ref * 'a globals_ram_scheme" where
-  "heap_new v s = 
+  "heap_new v s =
     (let p = new_pointer s;
          t = new_tag s in
     (\<lparr> pointer = p, tag = t \<rparr>,
@@ -276,7 +390,7 @@ lemma reborrow_update_heap: "\<lbrakk>wf_heap s; writable r s; reborrow r s = (r
   apply (erule reborrow_elims)
   apply (auto simp add: Let_def)
   using wf_tags_update apply simp
-  by (meson collect_tags_spec collect_tags_update in_mono set_ConsD)
+  by (meson collect_tags_spec collect_tags_update in_mono set_CosD)
 
 lemma reborrow_writable: "\<lbrakk>wf_heap s; writable r s; reborrow r s = (r', s')\<rbrakk> \<Longrightarrow> writable r s'"
   apply (erule reborrow_elims)
